@prefix dot: <https://w3id.org/dot#> .
@prefix bot: <https://w3id.org/bot#> .
@prefix owl: <http://www.w3.org/2002/07/owl#> .
@prefix rdf: <http://www.w3.org/1999/02/22-rdf-syntax-ns#> .
@prefix xsd: <http://www.w3.org/2001/XMLSchema#> .
@prefix brot: <https://wisib.de/ontologie/brot#> .
@prefix foaf: <http://xmlns.com/foaf/0.1/> .
@prefix rdfs: <http://www.w3.org/2000/01/rdf-schema#> .
@prefix voaf: <http://purl.org/vocommons/voaf#> .
@prefix vann: <http://purl.org/vocab/vann/> .
@prefix schema: <http://schema.org/#> .
@prefix dcterms: <http://purl.org/dc/terms/> .

<https://w3id.org/dot#> rdf:type owl:Ontology , voaf:Vocabulary ;
	dcterms:creator [
      rdf:type foaf:Person ;
      foaf:name "Al-Hakam Hamdan" ;
    ] ;
  dcterms:creator <https://www.researchgate.net/profile/Mathias_Bonduel> ;
  dcterms:contributor [
      rdf:type foaf:Person ;
      foaf:name "Mads Holten Rasmussen" ;
    ] ;
	owl:versionIRI <https://w3id.org/dot/0.8> ;
	owl:versionInfo "0.8" ;
	rdfs:comment """- Version 0.8: 
* completed ontology metadata wrt LOV
* added classes dot:ClassifiedDamage and dot:UnclassifiedDamage (subclasses of dot:Damage)
* made dot:StructuralDamage and dot:Defect subclasses of dot:Damage
"""@en ;
	dcterms:description "Ontology that defines the topology of damages in constructions."@en ;
	dcterms:license "https://creativecommons.org/licenses/by/1.0" ;
	dcterms:modified "2019-02-17"^^xsd:date ;
	dcterms:issued "2018-10-12"^^xsd:date ;
	dcterms:title "Damage Topology Ontology"@en ;
	vann:example "https://madsholten.github.io/sparql-visualizer/?file=https://raw.githubusercontent.com/Alhakam/dot/master/ABox-Examples/dot-demo.json"^^xsd:anyURI ;
	vann:example "https://raw.githubusercontent.com/Alhakam/dot/master/ABox-Examples/dotSampleData_pt1.ttl"^^xsd:anyURI ;
	vann:example "https://raw.githubusercontent.com/Alhakam/dot/master/ABox-Examples/dotSampleData_pt2.ttl"^^xsd:anyURI ;
	vann:preferredNamespacePrefix "dot" ;
	vann:preferredNamespaceUri "https://w3id.org/dot#" .

#################################################################
#    Object Properties
#################################################################

###  https://w3id.org/dot#adjacentDamageElement
dot:adjacentDamageElement rdf:type owl:ObjectProperty ,
                                   owl:SymmetricProperty ;
                          rdfs:domain dot:DamageElement ;
                          rdfs:range dot:DamageElement ;
                          rdfs:comment  "Defines the relationship between two instances of DamageElement that are physically connected with each other."@en ,
                                        "Definerer relationen mellem to Skadeselementer som er fysisk forbundet til hinanden."@da ;
                          rdfs:label    "adjacent DamageElement"@en ,
                                        "tilstødende Skadeselement"@da ;
						              rdfs:isDefinedBy dot: .


###  https://w3id.org/dot#aggregatesDamageElement
dot:aggregatesDamageElement rdf:type owl:ObjectProperty ;
                            rdfs:domain dot:DamageArea ;
                            rdfs:range dot:DamageElement ;
                            owl:propertyChainAxiom ( dot:aggregatesDamageElement
                                                     dot:adjacentDamageElement
                                                   ) ,
                                                   ( dot:aggregatesDamagePattern
                                                     dot:groupsDamageElement
                                                   ) ;
                            rdfs:comment  "A relationship between an instance of Damage Area and its consisting DamageElement instance."@en ,
                                          "En relation mellem et Skadeselement og det eller de Skadesområder som dette udgøres af."@da ;
                            rdfs:label    "aggregates Damage Element"@en ,
                                          "aggregerer Skadeselement"@da ;
							              rdfs:isDefinedBy dot: .


###  https://w3id.org/dot#aggregatesDamagePattern
dot:aggregatesDamagePattern rdf:type owl:ObjectProperty ;
                            rdfs:domain dot:DamageArea ;
                            rdfs:range dot:DamagePattern ;
                            rdfs:comment  "A relationship between an instance of DamageArea and its consisting DamagePattern instance."@en ,
                                          "En relation mellem et Skadesområde og det eller de Skademønstre som dette udgøres af."@da ;
                            rdfs:label    "aggregates Damage Pattern"@en ,
                                          "aggregerer Skademønster"@da ;
							              rdfs:isDefinedBy dot: .


###  https://w3id.org/dot#groupsDamageElement
dot:groupsDamageElement rdf:type owl:ObjectProperty ;
                        rdfs:domain dot:DamagePattern ;
                        rdfs:range dot:DamageElement ;
                        owl:propertyChainAxiom ( dot:groupsDamageElement
                                                 dot:adjacentDamageElement
                                               ) ;
                        rdfs:comment  "Groups instances of DamageElement that are physically connected in a DamagePattern."@en ,
                                      "Grupperer Skadeelementer som er fysisk forbundet i et Skademønster."@da ;
                        rdfs:label    "groups Damage Elements"@en ,
                                      "grupperer Skadeelement"@da ;
						            rdfs:isDefinedBy dot: .


###  https://w3id.org/dot#hasCausation
dot:hasCausation rdf:type owl:ObjectProperty ;
                 rdfs:domain dot:Damage ;
                 rdfs:range dot:Causation ;
                 rdfs:comment   "Relationship between a Damage and its Causation."@en ,
                                "Relation mellem en Skade og dens Forårsagelse."@da ;
                 rdfs:label     "has Causation"@en ,
                                "har Forårsagelse"@da ;
				         rdfs:isDefinedBy dot: .


###  https://w3id.org/dot#hasDamage
dot:hasDamage rdf:type owl:ObjectProperty ;
              rdfs:range dot:Damage ;
              schema:domainIncludes brot:BridgeElement ,
                                    brot:BridgeSpatialZone ,
                                    bot:Element ,
                                    bot:Zone ;
              rdfs:comment  "Defines the relationship between an affected component or structure (e.g. bot:Element) and a Damage."@en ,
                            "Definerer relationen mellem en påvirket bygningsdel eller konstruktion (fx bot:Element) og en Skade."@da ;
              rdfs:label    "has Damage"@en ,
                            "har Skade"@da ;
			        rdfs:isDefinedBy dot: .


###  https://w3id.org/dot#hasDamageArea
dot:hasDamageArea rdf:type owl:ObjectProperty ;
                  rdfs:subPropertyOf dot:hasDamage ;
                  rdfs:range dot:DamageArea ;
                  rdfs:comment  "Defines the relationship between an affected component or structure (e.g. bot:Element) and a DamageArea."@en ,
                                "Definerer relationen mellem en påvirket bygningsdel eller konstruktion (fx bot:Element) og et Skadesområde."@da ;
                  rdfs:label    "has DamageArea"@en ,
                                "har Skadesområde"@da ;
				          rdfs:isDefinedBy dot: .


###  https://w3id.org/dot#hasDamageElement
dot:hasDamageElement rdf:type owl:ObjectProperty ;
                     rdfs:subPropertyOf dot:hasDamage ;
                     rdfs:range dot:DamageElement ;
                     owl:propertyChainAxiom ( dot:hasDamageArea
                                              dot:aggregatesDamageElement
                                            ) ;
                     rdfs:comment "Defines the relationship between an affected component or structure (e.g. bot:Element) and a DamageElement."@en ,
                                  "Definerer relationen mellem en påvirket bygningsdel eller konstruktion (fx bot:Element) og et Skadeselement."@da ;
                     rdfs:label   "has DamageElement"@en ,
                                  "har Skadeselement"@da ;
					           rdfs:isDefinedBy dot: .


###  https://w3id.org/dot#coveredInDocumentation
dot:coveredInDocumentation rdf:type owl:ObjectProperty ;
                     rdfs:range dot:Documentation ;
                     schema:domainIncludes brot:BridgeElement ,
                                           brot:BridgeSpatialZone ,
                                           bot:Element ,
                                           bot:Zone ,
                                           dot:Damage ;
                     rdfs:comment "Relationship between a Documentation and the relevant documented or inspected object (e.g. dot:DamageArea or bot:Element). Should only be used for damage-relevant documentations."@en ,
                                  "Relation mellem en Dokumentation og det relevante dokumenterede eller inspicerede objekt (fx dot:DamageArea eller bot:Element). Bør kun benyttes for skadesrelevant dokumentation."@da ;
                     rdfs:label   "covered by documentation"@en ,
                                  "omfattet af dokumentation"@da ;
					           rdfs:isDefinedBy dot: .


###  https://w3id.org/dot#hasInspector
dot:hasInspector rdf:type owl:ObjectProperty ;
                 rdfs:domain dot:Inspection ;
                 rdfs:range dot:Inspector ;
                 rdfs:comment "Relationship between an Inspector and the Inspection that has been performed by him."@en ,
                              "Relation mellem en Inspektør og en Inspektion udført af denne person."@da ;
                 rdfs:label   "has Inspector"@en ,
                              "har Inspektør"@da ;
				         rdfs:isDefinedBy dot: .


###  https://w3id.org/dot#coveredByInspection
dot:coveredByInspection rdf:type owl:ObjectProperty ;
                        schema:domainIncludes dot:Damage ,
                                              brot:BridgeElement ,
                                              brot:BridgeSpatialZone ,
                                              bot:Element ,
                                              bot:Zone ;
                        rdfs:range dot:Inspection ;
                        owl:propertyChainAxiom ( dot:coveredInDocumentation
                                                 dot:documentationFromInspection
                                               ) ;
                        rdfs:comment "Relationship between a documented object (damage or component / zone) and the Inspection in which the object has been covered."@en ,
                                    "Relation mellem et dokumenteret objekt (skade eller komponent / zone) og Inspektionen hvoraf objektet er omfattet."@da ;
                        rdfs:label  "covered by inspection"@en ,
                                    "omfattet af inspektion"@da ;
                        rdfs:isDefinedBy dot: .


###  https://w3id.org/dot#hasDocumentation
dot:hasDocumentation rdf:type owl:ObjectProperty ;
                     owl:inverseOf dot:documentationFromInspection ;
                     rdfs:domain dot:Inspection ;
                     rdfs:range dot:Documentation ;
                     rdfs:comment "Relationship between an Inspection and the corresponding Documentation"@en ,
                                  "Relation mellem en Inspektion den tilhørende Dokumentation."@da ;
                     rdfs:label "has documentation"@en ,
                                "har dokumentation"@da ;
					           rdfs:isDefinedBy dot: .


###  https://w3id.org/dot#documentationFromInspection
dot:documentationFromInspection rdf:type owl:ObjectProperty ;
                    owl:inverseOf dot:hasDocumentation ;
                    rdfs:comment  "Relationship between a Documentation and the Inspection to which the Documentation refers. Inverse object property of dot:hasDocumentation."@en ,
                                  "Relation mellem en Dokumentation og Inspektionen som Dokumentationen refererer til. Omvendt objektegenskab af dot:hasDocumentation."@da ;
                    rdfs:label    "documentation from inspection"@en ,
                                  "dokumentation fra inspektion"@da ;
                    rdfs:isDefinedBy dot: .

#################################################################
#    Data properties
#################################################################

###  https://w3id.org/dot#filePath
dot:filePath rdf:type owl:DatatypeProperty ;
             rdfs:domain dot:ExternalResource ;
             rdfs:range xsd:anyURI ;
             rdfs:comment "Defines the unique location in a file system of an ExternalResource."@en ,
                          "Definerer en ekstern resources unikke sti i et filsystem."@da ;
             rdfs:label "file path"@en ,
                        "filsti"@da ;
             rdfs:isDefinedBy dot: .


###  https://w3id.org/dot#descriptionContent
dot:descriptionContent rdf:type owl:DatatypeProperty ;
                       rdfs:comment "Textual content used for the Description of a Structure Element or Damage."@en ,
                                  "Tekstbeskrivelse om en konstruktionsdel eller skade."@da ;
                       rdfs:label "description content"@en ,
                                  "beskrivelseskontekst"@da ;
                       rdfs:subPropertyOf dcterms:description ;
                       rdfs:isDefinedBy dot: ;
					   rdfs:range xsd:string ;
                       rdfs:domain dot:Description .


#################################################################
#    Classes
#################################################################

###  https://w3id.org/dot#Causation
dot:Causation rdf:type owl:Class ;
              rdfs:comment """Represents the causation of a damage.
Should be extended with domain-specific subclasses."""@en ,
                          """Repræsenterer skadens forårsagelse. 
Bør specificeres af en domæne-specifik underklasse."""@da ;
              rdfs:label  "Causation"@en ,
                          "Forårsagelse"@da ;
			        rdfs:isDefinedBy dot: .


###  https://w3id.org/dot#ClassifiedDamage
dot:ClassifiedDamage rdf:type owl:Class ;
			  rdfs:subClassOf dot:Damage ;
			  owl:disjointWith dot:UnclassifiedDamage ;
              rdfs:comment """A damage classification is used to denote the kind of damage. Subclasses of this class are defined in extensions 
			  such as CDO (Concrete Damage Ontology), NSO (the Natural Stone Ontology), etc."""@en ;
			  rdfs:isDefinedBy dot: ;
              rdfs:label "Classified Damage"@en .

###  https://w3id.org/dot#Damage
dot:Damage rdf:type owl:Class ;
           rdfs:comment """Damage is the harm to a structure resulting in impairment or loss of function, usefulness or value.
Instead of using dot:Damage, it is recommended to use one subclass of dot:Damage for respectively the damage topology (either dot:DamageArea or dot:DamageElement), the 
potential structural impact (either dot:StructuralDamage or dot:Defect) and the damage classification (either dot:UnclassifiedDamage or subclasses of dot:ClassifiedDamage)."""@en ,
                          """En Skade er en beskadigelse af en konstruktion, der resulterer i forringelse eller tab af funktion, nyttighed eller værdi.
I stedet for at benytte dot:Damage anbefales det at bruge en af underklasserne (enten dot:DamageArea eller dot:DamageElement)."""@da ;
           rdfs:label     "Damage"@en ,
                          "Skade"@da ;
           rdfs:isDefinedBy dot: .


###  https://w3id.org/dot#DamageArea
dot:DamageArea rdf:type owl:Class ;
               rdfs:subClassOf dot:Damage ;
               owl:disjointWith dot:DamageElement ,
                                dot:DamagePattern ;
               rdfs:comment "Area in a component where damage is located. Holds collection of multiple DamageElements or DamagePatterns. Used to be attached with simplified geometry."@en ,
                            "Område i et objekt hvor der er en beskadigelse. Beskriver en samling af et eller flere Skadeselementer eller Skadesmønstre. Kan tilknyttes simplificeret geometri."@da ;
               rdfs:label "Damage Area"@en ,
                          "Skadesområde"@da ;
               rdfs:isDefinedBy dot: .


###  https://w3id.org/dot#DamageElement
dot:DamageElement rdf:type owl:Class ;
              rdfs:subClassOf dot:Damage ;
              owl:disjointWith dot:DamagePattern ;
              rdfs:comment "Damage that is modeled on a very detailed level and belongs with other adjacent Damage Element instances to a broader damage area or damage pattern"@en ,
                            "En skade som er modelleret på et detaljeret niveau og hører sammen med andre tilstødende Skadeselementer i et større Skadesområde eller Skadesmønster."@da ;
              rdfs:label  "Damage Element"@en ,
                          "Skadeselement"@da ;
              rdfs:isDefinedBy dot: .


###  https://w3id.org/dot#DamagePattern
dot:DamagePattern rdf:type owl:Class ;
                  rdfs:comment "Defines a group of associated or physically connected instances of DamageElement. Used as class for grouping inside an instance of DamageArea."@en ,
                            "Definerer en gruppe af assosierede eller fysisk forbundne Skadesområder. Benyttes til at gruppere Skadesområder."@da ;
                  rdfs:label "Damage Pattern"@en ,
                          "Skadesmønster"@da ;
                  rdfs:isDefinedBy dot: .


###  https://w3id.org/dot#Defect
dot:Defect rdf:type owl:Class ;
		       rdfs:subClassOf dot:Damage ;
           owl:disjointWith dot:StructuralDamage ;
           rdfs:comment """Should be used on nodes that are already classified as dot:DamageArea or dot:DamageElement.
Damage that does not impair the structural integrity of the structure, but can still have influence on the durability, usability and / or value."""@en ,
                        """Benyttes på ting der allerede er klassificeret som et dot:DamageArea, dot:DamagePattern eller dot:DamageElement.
En Skade der ikke svækker den konstruktionsmæssige bæreevne, men som stadig har en indflydelse på holdbarheden, brugbarheden og / eller værdien."""@da ;
           rdfs:label     "Defect"@en ,
                          "Defekt"@da ;
           rdfs:isDefinedBy dot: .


###  https://w3id.org/dot#Description
dot:Description rdf:type owl:Class ;
                rdfs:subClassOf dot:Documentation ;
                rdfs:comment "Short textual documentation about a Damage or Structure Element. Generally created by the inspecting person."@en ,
                              "Kort tekstbeskrivelse om en Skade eller Konstruktionsdel. Typisk opretted af Inspektøren."@da ;
                rdfs:label "Description"@en ,
                          "Beskrivelse"@da ;
                rdfs:isDefinedBy dot: .


###  https://w3id.org/dot#Documentation
dot:Documentation rdf:type owl:Class ;
                  rdfs:comment "Material or data that provides information or evidence about the structure and its components or that serves as a record. Should only be used for damage-related documentation."@en ,
                              "Materiale eller data der tilvejebringer information eller bevis om konstruktionen og dens bestanddele eller som fungerer som journal. Bør kun benyttes for skadesrelateret dokumentation."@da ;
                  rdfs:label "Damage Documentation"@en ,
                          "Skadesdokumentation"@da ;
                  rdfs:isDefinedBy dot: .


###  https://w3id.org/dot#ExternalResource
dot:ExternalResource rdf:type owl:Class ;
                     rdfs:subClassOf dot:Documentation ;
                     rdfs:comment "Document that is stored in a separate file, referenced by an external path."@en ,
                                  "Dokument der gemmes i en seperat fil, refereret af en ekstern sti."@da ;
                     rdfs:label "External Resource"@en ,
                          "Ekstern Resource"@da ;
                     rdfs:isDefinedBy dot: .


###  https://w3id.org/dot#Inspection
dot:Inspection rdf:type owl:Class ;
               rdfs:comment """Careful examination or scrutiny in which an existing construction or a part of it is inspected and detected damages are recorded.
Should be repeated at regular time intervals."""@en ,
                            """Omhyggelig undersøgelse eller granskning hvori en eksisterende konstruktion eller en del ad denne inspiceres og detekterede beskadigelser registreres.
Inspektioner bør udføres regelmæssigt."""@da ;
               rdfs:label "Inspection"@en ,
                          "Inspektion"@da ;
               rdfs:isDefinedBy dot: .


###  https://w3id.org/dot#Inspector
dot:Inspector rdf:type owl:Class ;
              rdfs:subClassOf foaf:Person ;
              rdfs:comment "A person who inspects constructions (for damages) or whose task it is to carry out inspections on constructions."@en ,
                            "En person der inspicerer konstruktioner (for skader) eller hvis opgave er at udføre inspektioner af konstruktioner."@da ;
              rdfs:label  "Inspector"@en ,
                          "Inspektør"@da ;
              rdfs:isDefinedBy dot: .


###  https://w3id.org/dot#StructuralDamage
dot:StructuralDamage rdf:type owl:Class ;
                     rdfs:comment """Should be used on nodes that are already classified as dot:DamageArea, dot:DamagePattern or dot:DamageElement.
Damage that impairs the structural integrity of the structure."""@en ,
                                  """Benyttes på ting der allerede er klassificeret som et dot:DamageArea, dot:DamagePattern eller dot:DamageElement.
En Skade der svækker den konstruktionsmæssige bæreevne."""@da ;
                     rdfs:label "Structural Damage"@en ,
                          "Konstruktionsmæssig Skade"@da ;
					           rdfs:subClassOf dot:Damage ;
                     rdfs:isDefinedBy dot: .


###  https://w3id.org/dot#UnclassifiedDamage
dot:UnclassifiedDamage rdf:type owl:Class ;
					   rdfs:subClassOf dot:Damage ;
                       rdfs:comment """A dot:Damage instance that is not further classified with domain-specific classes (subclasses of dot:ClassifiedDamage). 
This class can be used in cases where the damage classification is unknown."""@en ;
                       rdfs:isDefinedBy dot: ;
					   rdfs:label "Unclassified Damage"@en .
